

Lambda Calculus Constructions

Greyson Knippel

CPSC 326-01 — Gonzaga University, compiled with \LaTeX

Professor Johnson

January 23, 2026

to start off:

$$\text{SUCC } X = X + 1$$

$$\text{PRED } X = X - 1$$

$$(= X Y) \Rightarrow \text{T/F}$$

construction of ADD

using recursion: R , ADD can be defined as:

$$\begin{aligned} R \text{ ADD } X Y &= R \text{ ADD } X Y \\ &= (\text{if } (= Y 0) (\text{then}) X (\text{else}) (\text{ADD } (\text{SUCC } X) (\text{PRED } Y))) \end{aligned}$$

construction of MULT

MULT can also be defined by using recursion R : but this time its simply just repeated addition.

$$\begin{aligned} R \text{ MULT } X Y &= R \text{ MULT } X Y \\ &= (\text{if } (= Y 0) (\text{then}) 0 (\text{else}) (\text{ADD } X (\text{MULT } X (\text{PRED } Y)))) \end{aligned}$$

example — ADD 2 3

R ADD 2 3 = (if) (= 3 0) 2 (ADD (SUCC 2) (PRED 3))
= (if) (= 2 0) 3 (ADD (SUCC 3) (PRED 2))
= (if) (= 1 0) 4 (ADD (SUCC 4) (PRED 1))
= (if) (= 0 0) 5 (ADD (SUCC 5) (PRED 0))

- basically (= y 0) is your base case,
then use recursion with SUCC AND PRED.

= 5

example — MULT 2 4

MULT 2 4 = (if) (= 4 0) (then) 0 (else) (ADD 2 (MULT 2 (PRED 4)))
= (if) (= 3 0) (then) 0 (else) (ADD 2 (MULT 2 (PRED 3)))
= (if) (= 2 0) (then) 0 (else) (ADD 2 (MULT 2 (PRED 2)))
= (if) (= 1 0) (then) 0 (else) (ADD 2 (MULT 2 (PRED 1)))
= (if) (= 0 0) (then) 0 (else) (ADD 2 (MULT 2 (PRED 0)))

and adding all the recursions together with the ADD block...

- basically we are just using ADD's recursion,
doing repeated addition with MULT's recursion.

= 8